code/bignum/Hacl.Impl.Exponentiation.fsti
@@ -8,13 +8,8 @@ open Lib.IntTypes
 open Lib.Buffer
 
 module ST = FStar.HyperStack.ST
-module B = LowStar.Buffer
-
 module LSeq = Lib.Sequence
-module BSeq = Lib.ByteSequence
-module Loops = Lib.LoopCombinators
 
-module LE = Lib.Exponentiation
 module SE = Spec.Exponentiation
 module BD = Hacl.Bignum.Definitions
 
@@ -97,6 +92,8 @@ class concrete_ops (a_t:inttype_a) (len:size_t{v len > 0}) (ctx_len:size_t) = {
 }
 
 
+// This function computes `a^b` using a binary right-to-left method
+// It takes variable time to compute the result
 inline_for_extraction noextract
 val lexp_rl_vartime:
     #a_t:inttype_a
@@ -124,6 +121,8 @@ val lexp_rl_vartime:
     SE.exp_rl #k.to.t_spec k.to.concr_ops (k.to.refl (as_seq h0 a)) (v bBits) (BD.bn_v h0 b))
 
 
+// This function computes `a^b` using Montgomery's ladder (a binary method)
+// It takes constant time to compute the result
 inline_for_extraction noextract
 val lexp_mont_ladder_swap_consttime:
     #a_t:inttype_a
@@ -151,6 +150,7 @@ val lexp_mont_ladder_swap_consttime:
     SE.exp_mont_ladder_swap #k.to.t_spec k.to.concr_ops (k.to.refl (as_seq h0 a)) (v bBits) (BD.bn_v h0 b))
 
 
+// This function computes `a^(2^b)` and writes the result in `res`
 inline_for_extraction noextract
 val lexp_pow2:
     #a_t:inttype_a
@@ -170,8 +170,9 @@ val lexp_pow2:
     k.to.refl (as_seq h1 res) == SE.exp_pow2 k.to.concr_ops (k.to.refl (as_seq h0 a)) (v b))
 
 
+// This function computes `acc^(2^b)` and writes the result in `acc`
 inline_for_extraction noextract
-val lexp_pow_in_place:
+val lexp_pow2_in_place:
     #a_t:inttype_a
   -> len:size_t{v len > 0}
   -> ctx_len:size_t
@@ -188,7 +189,153 @@ val lexp_pow_in_place:
 
 
 inline_for_extraction noextract
-let lexp_fw_st (a_t:inttype_a) (len:size_t{v len > 0}) (ctx_len:size_t) (k:concrete_ops a_t len ctx_len) =
+let precomp_table_inv
+  (#a_t:inttype_a)
+  (len:size_t{v len > 0})
+  (ctx_len:size_t)
+  (k:concrete_ops a_t len ctx_len)
+  (a:LSeq.lseq (uint_t a_t SEC) (v len))
+  (table_len:size_t{v table_len * v len <= max_size_t})
+  (table:LSeq.lseq (uint_t a_t SEC) (v table_len * v len))
+  (j:nat{j < v table_len}) : Type0
+ =
+  Math.Lemmas.lemma_mult_le_right (v len) (j + 1) (v table_len);
+  let bj = LSeq.sub table (j * v len) (v len) in
+  k.to.linv bj /\ k.to.linv a /\
+  k.to.refl bj == SE.pow k.to.concr_ops (k.to.refl a) j
+
+
+// This function computes [a^0 = one; a^1; a^2; ..; a^(table_len - 1)]
+inline_for_extraction noextract
+val lprecomp_table:
+    #a_t:inttype_a
+  -> len:size_t{v len > 0}
+  -> ctx_len:size_t
+  -> k:concrete_ops a_t len ctx_len
+  -> ctx:lbuffer (uint_t a_t SEC) ctx_len
+  -> a:lbuffer (uint_t a_t SEC) len
+  -> table_len:size_t{1 < v table_len /\ v table_len * v len <= max_size_t}
+  -> table:lbuffer (uint_t a_t SEC) (table_len *! len) ->
+  Stack unit
+  (requires fun h ->
+    live h a /\ live h table /\ live h ctx /\
+    disjoint a table /\ disjoint ctx table /\ disjoint a ctx /\
+    k.to.linv (as_seq h a) /\ k.to.linv_ctx (as_seq h ctx) /\
+    k.to.linv (as_seq h (gsub table 0ul len)) /\
+    k.to.refl (as_seq h (gsub table 0ul len)) == k.to.concr_ops.SE.one ())
+  (ensures  fun h0 _ h1 -> modifies (loc table) h0 h1 /\
+    (forall (j:nat{j < v table_len}).{:pattern precomp_table_inv len ctx_len k (as_seq h1 a) table_len (as_seq h1 table) j}
+      precomp_table_inv len ctx_len k (as_seq h1 a) table_len (as_seq h1 table) j))
+
+
+inline_for_extraction noextract
+let lprecomp_get_st
+  (a_t:inttype_a)
+  (len:size_t{v len > 0})
+  (ctx_len:size_t)
+  (k:concrete_ops a_t len ctx_len) =
+    a:lbuffer (uint_t a_t SEC) len
+  -> table_len:size_t{1 < v table_len /\ v table_len * v len <= max_size_t}
+  -> table:lbuffer (uint_t a_t SEC) (table_len *! len)
+  -> bits_l:uint_t a_t SEC{v bits_l < v table_len}
+  -> tmp:lbuffer (uint_t a_t SEC) len ->
+  Stack unit
+  (requires fun h ->
+    live h a /\ live h table /\ live h tmp /\
+    disjoint a table /\ disjoint a tmp /\ disjoint table tmp /\
+    k.to.linv (as_seq h a) /\
+    (forall (j:nat{j < v table_len}).
+      precomp_table_inv len ctx_len k (as_seq h a) table_len (as_seq h table) j))
+  (ensures  fun h0 _ h1 -> modifies (loc tmp) h0 h1 /\
+    k.to.linv (as_seq h1 tmp) /\
+    k.to.refl (as_seq h1 tmp) == SE.pow k.to.concr_ops (k.to.refl (as_seq h0 a)) (v bits_l))
+
+
+// This function returns table.[bits_l] = a^bits_l
+// It takes variable time to access bits_l-th element of a table
+inline_for_extraction noextract
+val lprecomp_get_vartime:
+     #a_t:inttype_a
+  -> len:size_t{v len > 0}
+  -> ctx_len:size_t
+  -> k:concrete_ops a_t len ctx_len ->
+  lprecomp_get_st a_t len ctx_len k
+
+
+// This function returns table.[bits_l] = a^bits_l
+// It takes constant time to access bits_l-th element of a table
+inline_for_extraction noextract
+val lprecomp_get_consttime:
+     #a_t:inttype_a
+  -> len:size_t{v len > 0}
+  -> ctx_len:size_t
+  -> k:concrete_ops a_t len ctx_len ->
+  lprecomp_get_st a_t len ctx_len k
+
+
+inline_for_extraction noextract
+let lexp_fw_table_st
+  (a_t:inttype_a)
+  (len:size_t{v len > 0})
+  (ctx_len:size_t)
+  (k:concrete_ops a_t len ctx_len) =
+    ctx:lbuffer (uint_t a_t SEC) ctx_len
+  -> a:lbuffer (uint_t a_t SEC) len
+  -> bLen:size_t
+  -> bBits:size_t{(v bBits - 1) / bits a_t < v bLen}
+  -> b:lbuffer (uint_t a_t SEC) bLen
+  -> l:size_t{0 < v l /\ v l < bits a_t /\ v l < 32}
+  -> table_len:size_t{1 < v table_len /\ v table_len * v len <= max_size_t /\ v table_len == pow2 (v l)}
+  -> table:lbuffer (uint_t a_t SEC) (table_len *! len)
+  -> acc:lbuffer (uint_t a_t SEC) len ->
+  Stack unit
+  (requires fun h ->
+    live h a /\ live h b /\ live h acc /\ live h ctx /\ live h table /\
+    disjoint a acc /\ disjoint a ctx /\ disjoint a table /\ disjoint b acc /\
+    disjoint acc ctx /\ disjoint acc table /\ disjoint ctx table /\
+    BD.bn_v h b < pow2 (v bBits) /\
+    k.to.linv_ctx (as_seq h ctx) /\ k.to.linv (as_seq h a) /\
+    k.to.linv (as_seq h acc) /\ k.to.refl (as_seq h acc) == k.to.concr_ops.SE.one () /\
+    (forall (j:nat{j < v table_len}).
+      precomp_table_inv len ctx_len k (as_seq h a) table_len (as_seq h table) j))
+  (ensures  fun h0 _ h1 -> modifies (loc acc) h0 h1 /\
+    k.to.linv (as_seq h1 acc) /\
+    k.to.refl (as_seq h1 acc) ==
+    SE.exp_fw k.to.concr_ops (k.to.refl (as_seq h0 a)) (v bBits) (BD.bn_v h0 b) (v l))
+
+
+// This function computes `a^b` using a fixed-window method
+// It takes variable time to compute the result
+// The function also expects a precomputed table for `a`, i.e.,
+// table = [a^0 = one; a^1; a^2; ..; a^(table_len - 1)]
+inline_for_extraction noextract
+val lexp_fw_table_vartime:
+    #a_t:inttype_a
+  -> len:size_t{v len > 0}
+  -> ctx_len:size_t
+  -> k:concrete_ops a_t len ctx_len ->
+  lexp_fw_table_st a_t len ctx_len k
+
+
+// This function computes `a^b` using a fixed-window method
+// It takes constant time to compute the result
+// The function also expects a precomputed table for `a`, i.e.,
+// table = [a^0 = one; a^1; a^2; ..; a^(table_len - 1)]
+inline_for_extraction noextract
+val lexp_fw_table_consttime:
+    #a_t:inttype_a
+  -> len:size_t{v len > 0}
+  -> ctx_len:size_t
+  -> k:concrete_ops a_t len ctx_len ->
+  lexp_fw_table_st a_t len ctx_len k
+
+
+inline_for_extraction noextract
+let lexp_fw_st
+  (a_t:inttype_a)
+  (len:size_t{v len > 0})
+  (ctx_len:size_t)
+  (k:concrete_ops a_t len ctx_len) =
     ctx:lbuffer (uint_t a_t SEC) ctx_len
   -> a:lbuffer (uint_t a_t SEC) len
   -> bLen:size_t
@@ -211,6 +358,8 @@ let lexp_fw_st (a_t:inttype_a) (len:size_t{v len > 0}) (ctx_len:size_t) (k:concr
     SE.exp_fw #k.to.t_spec k.to.concr_ops (k.to.refl (as_seq h0 a)) (v bBits) (BD.bn_v h0 b) (v l))
 
 
+// This function computes `a^b` using a fixed-window method
+// It takes variable time to compute the result
 inline_for_extraction noextract
 val lexp_fw_vartime:
     #a_t:inttype_a
@@ -220,6 +369,8 @@ val lexp_fw_vartime:
   lexp_fw_st a_t len ctx_len k
 
 
+// This function computes `a^b` using a fixed-window method
+// It takes constant time to compute the result
 inline_for_extraction noextract
 val lexp_fw_consttime:
     #a_t:inttype_a
