code/bignum/Hacl.Impl.MultiExponentiation.fst
@@ -8,19 +8,9 @@ open Lib.IntTypes
 open Lib.Buffer
 
 module ST = FStar.HyperStack.ST
-module B = LowStar.Buffer
-
-module LSeq = Lib.Sequence
-module BSeq = Lib.ByteSequence
 module Loops = Lib.LoopCombinators
-
-module LE = Lib.Exponentiation
 module SE = Spec.Exponentiation
 module BD = Hacl.Bignum.Definitions
-module BN = Hacl.Bignum
-module SN = Hacl.Spec.Bignum
-module BB = Hacl.Bignum.Base
-module SB = Hacl.Spec.Bignum.Base
 
 friend Hacl.Impl.Exponentiation
 
@@ -232,66 +222,32 @@ let lexp_double_fw_loop #a_t len ctx_len k lprecomp_get ctx a1 bLen bBits b1 a2 
 
 
 inline_for_extraction noextract
-let lexp_double_fw_gen_st
-  (a_t:inttype_a)
-  (len:size_t{v len > 0})
-  (ctx_len:size_t)
-  (k:concrete_ops a_t len ctx_len) =
-    ctx:lbuffer (uint_t a_t SEC) ctx_len
-  -> a1:lbuffer (uint_t a_t SEC) len
-  -> bLen:size_t
-  -> bBits:size_t{(v bBits - 1) / bits a_t < v bLen}
-  -> b1:lbuffer (uint_t a_t SEC) bLen
-  -> a2:lbuffer (uint_t a_t SEC) len
-  -> b2:lbuffer (uint_t a_t SEC) bLen
-  -> l:size_t{0 < v l /\ v l < bits a_t /\ v l < 32}
-  -> table_len:size_t{1 < v table_len /\ v table_len * v len <= max_size_t /\ v table_len == pow2 (v l)}
-  -> table1:lbuffer (uint_t a_t SEC) (table_len *! len)
-  -> table2:lbuffer (uint_t a_t SEC) (table_len *! len)
-  -> acc:lbuffer (uint_t a_t SEC) len ->
-  Stack unit
-  (requires fun h ->
-    live h a1 /\ live h b1 /\ live h a2 /\ live h b2 /\
-    live h acc /\ live h ctx /\ live h table1 /\ live h table2 /\
-
-    eq_or_disjoint a1 a2 /\ disjoint a1 acc /\ disjoint a1 ctx /\
-    disjoint a1 table1 /\ disjoint a1 table2 /\ disjoint b1 acc /\
-    disjoint a2 acc /\ disjoint a2 ctx /\ disjoint a2 table1 /\ disjoint a2 table2 /\
-    disjoint b2 acc /\ disjoint acc ctx /\ disjoint acc table1 /\ disjoint acc table2 /\
-    disjoint ctx table1 /\ disjoint ctx table2 /\ eq_or_disjoint table1 table2 /\
-
-    BD.bn_v h b1 < pow2 (v bBits) /\
-    BD.bn_v h b2 < pow2 (v bBits) /\
-    k.to.linv_ctx (as_seq h ctx) /\
-    k.to.linv (as_seq h a1) /\ k.to.linv (as_seq h a2) /\
-    k.to.linv (as_seq h acc) /\ k.to.refl (as_seq h acc) == k.to.concr_ops.SE.one () /\
-    (forall (j:nat{j < v table_len}).
-      precomp_table_inv len ctx_len k (as_seq h a1) table_len (as_seq h table1) j) /\
-    (forall (j:nat{j < v table_len}).
-      precomp_table_inv len ctx_len k (as_seq h a2) table_len (as_seq h table2) j))
-  (ensures  fun h0 _ h1 -> modifies (loc acc) h0 h1 /\
-    k.to.linv (as_seq h1 acc) /\
-    k.to.refl (as_seq h1 acc) ==
-    SE.exp_double_fw k.to.concr_ops
-      (k.to.refl (as_seq h0 a1)) (v bBits) (BD.bn_v h0 b1)
-      (k.to.refl (as_seq h0 a2)) (BD.bn_v h0 b2) (v l))
-
-
-inline_for_extraction noextract
-val lexp_double_fw_gen_:
+val lexp_double_fw_tables_gen:
     #a_t:inttype_a
   -> len:size_t{v len > 0}
   -> ctx_len:size_t
   -> k:concrete_ops a_t len ctx_len
   -> lprecomp_get:lprecomp_get_st a_t len ctx_len k ->
-  lexp_double_fw_gen_st a_t len ctx_len k
+  lexp_double_fw_tables_st a_t len ctx_len k
 
-let lexp_double_fw_gen_ #a_t len ctx_len k lprecomp_get ctx a1 bLen bBits b1 a2 b2 l table_len table1 table2 acc =
+let lexp_double_fw_tables_gen #a_t len ctx_len k lprecomp_get ctx a1 bLen bBits b1 a2 b2 l table_len table1 table2 acc =
   assert (v (bBits %. l) == v bBits % v l);
   if bBits %. l <> 0ul then
     lexp_double_fw_acc0 len ctx_len k lprecomp_get ctx a1 bLen bBits b1 a2 b2 l table_len table1 table2 acc;
 
   lexp_double_fw_loop #a_t len ctx_len k lprecomp_get ctx a1 bLen bBits b1 a2 b2 l table_len table1 table2 acc
+
+
+let lexp_double_fw_tables_vartime #a_t len ctx_len k ctx a1 bLen bBits b1 a2 b2 l table_len table1 table2 acc =
+  lexp_double_fw_tables_gen #a_t len ctx_len k
+    (lprecomp_get_vartime #a_t len ctx_len k)
+    ctx a1 bLen bBits b1 a2 b2 l table_len table1 table2 acc
+
+
+let lexp_double_fw_tables_consttime #a_t len ctx_len k ctx a1 bLen bBits b1 a2 b2 l table_len table1 table2 acc =
+  lexp_double_fw_tables_gen #a_t len ctx_len k
+    (lprecomp_get_consttime #a_t len ctx_len k)
+    ctx a1 bLen bBits b1 a2 b2 l table_len table1 table2 acc
 
 
 inline_for_extraction noextract
@@ -329,19 +285,19 @@ let lexp_double_fw_gen #a_t len ctx_len k lprecomp_get ctx a1 bLen bBits b1 a2 b
   assert (forall (j:nat{j < v table_len}).
       precomp_table_inv len ctx_len k (as_seq h a2) table_len (as_seq h table2) j);
 
-  lexp_double_fw_gen_ #a_t len ctx_len k lprecomp_get
+  lexp_double_fw_tables_gen #a_t len ctx_len k lprecomp_get
     ctx a1 bLen bBits b1 a2 b2 l table_len table1 table2 acc;
   pop_frame ()
 #pop-options
 
 
-let lexp_double_fw_vartime #a_t len ctx_len k ctx a1 bLen bBits b1 a2 b2 acc w =
+let lexp_double_fw_vartime #a_t len ctx_len k ctx a1 bLen bBits b1 a2 b2 acc l =
   lexp_double_fw_gen #a_t len ctx_len k
     (lprecomp_get_vartime #a_t len ctx_len k)
-    ctx a1 bLen bBits b1 a2 b2 acc w
+    ctx a1 bLen bBits b1 a2 b2 acc l
 
 
-let lexp_double_fw_consttime #a_t len ctx_len k ctx a1 bLen bBits b1 a2 b2 acc w =
+let lexp_double_fw_consttime #a_t len ctx_len k ctx a1 bLen bBits b1 a2 b2 acc l =
   lexp_double_fw_gen #a_t len ctx_len k
     (lprecomp_get_consttime #a_t len ctx_len k)
-    ctx a1 bLen bBits b1 a2 b2 acc w
+    ctx a1 bLen bBits b1 a2 b2 acc l
