code/bignum/Hacl.Impl.MultiExponentiation.fsti
@@ -8,13 +8,6 @@ open Lib.IntTypes
 open Lib.Buffer
 
 module ST = FStar.HyperStack.ST
-module B = LowStar.Buffer
-
-module LSeq = Lib.Sequence
-module BSeq = Lib.ByteSequence
-module Loops = Lib.LoopCombinators
-
-module LE = Lib.Exponentiation
 module SE = Spec.Exponentiation
 module BD = Hacl.Bignum.Definitions
 
@@ -23,7 +16,85 @@ open Hacl.Impl.Exponentiation
 #reset-options "--z3rlimit 50 --fuel 0 --ifuel 0"
 
 inline_for_extraction noextract
-let lexp_double_fw_st (a_t:inttype_a) (len:size_t{v len > 0}) (ctx_len:size_t) (k:concrete_ops a_t len ctx_len) =
+let lexp_double_fw_tables_st
+  (a_t:inttype_a)
+  (len:size_t{v len > 0})
+  (ctx_len:size_t)
+  (k:concrete_ops a_t len ctx_len) =
+    ctx:lbuffer (uint_t a_t SEC) ctx_len
+  -> a1:lbuffer (uint_t a_t SEC) len
+  -> bLen:size_t
+  -> bBits:size_t{(v bBits - 1) / bits a_t < v bLen}
+  -> b1:lbuffer (uint_t a_t SEC) bLen
+  -> a2:lbuffer (uint_t a_t SEC) len
+  -> b2:lbuffer (uint_t a_t SEC) bLen
+  -> l:size_t{0 < v l /\ v l < bits a_t /\ v l < 32}
+  -> table_len:size_t{1 < v table_len /\ v table_len * v len <= max_size_t /\ v table_len == pow2 (v l)}
+  -> table1:lbuffer (uint_t a_t SEC) (table_len *! len)
+  -> table2:lbuffer (uint_t a_t SEC) (table_len *! len)
+  -> acc:lbuffer (uint_t a_t SEC) len ->
+  Stack unit
+  (requires fun h ->
+    live h a1 /\ live h b1 /\ live h a2 /\ live h b2 /\
+    live h acc /\ live h ctx /\ live h table1 /\ live h table2 /\
+
+    eq_or_disjoint a1 a2 /\ disjoint a1 acc /\ disjoint a1 ctx /\
+    disjoint a1 table1 /\ disjoint a1 table2 /\ disjoint b1 acc /\
+    disjoint a2 acc /\ disjoint a2 ctx /\ disjoint a2 table1 /\ disjoint a2 table2 /\
+    disjoint b2 acc /\ disjoint acc ctx /\ disjoint acc table1 /\ disjoint acc table2 /\
+    disjoint ctx table1 /\ disjoint ctx table2 /\ eq_or_disjoint table1 table2 /\
+
+    BD.bn_v h b1 < pow2 (v bBits) /\
+    BD.bn_v h b2 < pow2 (v bBits) /\
+    k.to.linv_ctx (as_seq h ctx) /\
+    k.to.linv (as_seq h a1) /\ k.to.linv (as_seq h a2) /\
+    k.to.linv (as_seq h acc) /\ k.to.refl (as_seq h acc) == k.to.concr_ops.SE.one () /\
+    (forall (j:nat{j < v table_len}).
+      precomp_table_inv len ctx_len k (as_seq h a1) table_len (as_seq h table1) j) /\
+    (forall (j:nat{j < v table_len}).
+      precomp_table_inv len ctx_len k (as_seq h a2) table_len (as_seq h table2) j))
+  (ensures  fun h0 _ h1 -> modifies (loc acc) h0 h1 /\
+    k.to.linv (as_seq h1 acc) /\
+    k.to.refl (as_seq h1 acc) ==
+    SE.exp_double_fw k.to.concr_ops
+      (k.to.refl (as_seq h0 a1)) (v bBits) (BD.bn_v h0 b1)
+      (k.to.refl (as_seq h0 a2)) (BD.bn_v h0 b2) (v l))
+
+
+// This function computes `a1^b1 `mul` a2^b2` using a fixed-window method
+// It takes variable time to compute the result
+// The function also expects precomputed tables for `a1` and `a2`, i.e.,
+// table1 = [a1^0 = one; a1^1; a1^2; ..; a1^(table_len - 1)]
+// table2 = [a2^0 = one; a2^1; a2^2; ..; a2^(table_len - 1)]
+inline_for_extraction noextract
+val lexp_double_fw_tables_vartime:
+    #a_t:inttype_a
+  -> len:size_t{v len > 0}
+  -> ctx_len:size_t
+  -> k:concrete_ops a_t len ctx_len ->
+  lexp_double_fw_tables_st a_t len ctx_len k
+
+
+// This function computes `a1^b1 `mul` a2^b2` using a fixed-window method
+// It takes constant time to compute the result
+// The function also expects precomputed tables for `a1` and `a2`, i.e.,
+// table1 = [a1^0 = one; a1^1; a1^2; ..; a1^(table_len - 1)]
+// table2 = [a2^0 = one; a2^1; a2^2; ..; a2^(table_len - 1)]
+inline_for_extraction noextract
+val lexp_double_fw_tables_consttime:
+    #a_t:inttype_a
+  -> len:size_t{v len > 0}
+  -> ctx_len:size_t
+  -> k:concrete_ops a_t len ctx_len ->
+  lexp_double_fw_tables_st a_t len ctx_len k
+
+
+inline_for_extraction noextract
+let lexp_double_fw_st
+  (a_t:inttype_a)
+  (len:size_t{v len > 0})
+  (ctx_len:size_t)
+  (k:concrete_ops a_t len ctx_len) =
     ctx:lbuffer (uint_t a_t SEC) ctx_len
   -> a1:lbuffer (uint_t a_t SEC) len
   -> bLen:size_t
@@ -52,6 +123,8 @@ let lexp_double_fw_st (a_t:inttype_a) (len:size_t{v len > 0}) (ctx_len:size_t) (
       (k.to.refl (as_seq h0 a2)) (BD.bn_v h0 b2) (v l))
 
 
+// This function computes `a1^b1 `mul` a2^b2` using a fixed-window method
+// It takes variable time to compute the result
 inline_for_extraction noextract
 val lexp_double_fw_vartime:
     #a_t:inttype_a
@@ -61,6 +134,8 @@ val lexp_double_fw_vartime:
   lexp_double_fw_st a_t len ctx_len k
 
 
+// This function computes `a1^b1 `mul` a2^b2` using a fixed-window method
+// It takes constant time to compute the result
 inline_for_extraction noextract
 val lexp_double_fw_consttime:
     #a_t:inttype_a
